build.sh
@@ -3,5 +3,5 @@
 eval $(opam env)
 
 coq_makefile -f _CoqProject -o CoqMakefile
-
+make -f CoqMakefile install
 make -f CoqMakefile
